lntps.v
@@ -1,0 +1,101 @@
+
+(* try non-adjacent exchange, for system with princrule and seqrule *)
+
+Require Import lnt.
+
+Definition can_gen_exchL (V : Set)
+  (rules : rls (list (rel (list (PropF V)) * dir))) ns :=
+  forall G H seq (d : dir) Γ1 Γ2 Γ3 (A B : PropF V) Δ,
+  ns = G ++ (seq, d) :: H -> seq = pair (Γ1 ++ A :: Γ2 ++ B :: Γ3) Δ ->
+  derrec rules (fun _ => False) 
+    (G ++ (pair (Γ1 ++ B :: Γ2 ++ A :: Γ3) Δ, d) :: H).
+
+
+
+Lemma gen_exchL: forall (V : Set) ns
+  (D : derrec (nsrule (seqrule (@princrule V))) (fun _ => False) ns),
+  can_gen_exchL (nsrule (seqrule (@princrule V))) ns.
+
+Proof.
+intro.  intro.  intro.
+eapply derrec_all_ind in D.
+exact D. tauto.
+intros. inversion H.  unfold nsext in H5.
+unfold can_gen_exchL.  intros.
+unfold nsext in H7.
+(* cases of where the exchange occurs vs where the last rule applied *)
+apply partition_2_2 in H7.
+remember (Γ1 ++ B :: Γ2 ++ A :: Γ3, Δ) as seqe.
+
+decompose [or] H7. clear H7.  cE.
+(* case where the rule is applied in a sequent to the right
+  of where the exchange takes place *)
+remember (G0 ++ (seqe, d0) :: x) as Ge.
+remember (map (nsext Ge H2 d) ps0) as pse.
+
+apply derI with pse. subst pse. subst H6.
+rewrite list_rearr14.
+(* it must be easier than this
+  to rewrite using the inverse of the definition of nsext *)
+rewrite <- nsext_def.  subst seqe.  rewrite <- HeqGe.
+apply NSctxt. assumption.
+
+rewrite dersrec_all.  rewrite Forall_forall.
+intros q qin.  subst pse.  rewrite in_map_iff in qin. cE.
+subst q.  clear H0 H.  subst ps.
+rewrite Forall_forall in H1.
+rename_last inps0.  eapply in_map in inps0. pose (H1 _ inps0).
+unfold can_gen_exchL in c0.
+unfold nsext. subst Ge. subst seqe.
+rewrite <- list_rearr14.
+eapply c0. 2:reflexivity.
+unfold nsext. subst G. subst seq.
+list_eq_assoc.
+
+all : revgoals. clear H7. cE.
+(* now the case where the rule is applied in a sequent to the left
+  of where the exchange takes place *)
+remember (x ++ (seqe, d0) :: H6) as He.
+remember (map (nsext G He d) ps0) as pse.
+
+apply derI with pse. subst pse. subst G0.
+rewrite <- list_rearr14.
+(* it must be easier than this
+  to rewrite using the inverse of the definition of nsext *)
+rewrite <- nsext_def.  subst seqe.  rewrite <- HeqHe.
+apply NSctxt. assumption.
+
+rewrite dersrec_all.  rewrite Forall_forall.
+intros q qin.  subst pse.  rewrite in_map_iff in qin. cE.
+subst q.  clear H0 H.  subst ps.
+rewrite Forall_forall in H1.
+rename_last inps0.  eapply in_map in inps0. pose (H1 _ inps0).
+unfold can_exchL in c0.
+unfold nsext. subst He. subst seqe.
+rewrite list_rearr14.
+
+eapply c0. 2:reflexivity.
+unfold nsext. subst H2. subst seq.
+apply list_rearr14.
+
+(* now case where exchange and rule application occur in the same sequent *)
+cE. clear H7. injection H10 as.
+inversion H3 as [? ? ? ? ? ? pr mse se].
+unfold seqext in se.
+subst.  clear H. clear H3.
+destruct c0. unfold seqext in se.
+injection se as sel ser.
+subst.  inversion pr. subst.
+(* case of Id rule *)
+apply derI with [].  2: apply dlNil.
+rewrite <- nsext_def. apply NSctxt_nil.
+acacD ; subst ; list_assoc_r_simp ; list_app_nil.
+
+
+
+  repeat (rewrite <- !app_assoc || rewrite <- !app_comm_cons) ;
+  repeat (apply Id || rewrite list_rearr16 || rewrite list_rearr15).
+
+
+
+
